Foundation/Propositional/Kripke/Basic.lean
@@ -35,14 +35,33 @@ lemma rel_antisymm' : x ≺ y → y ≺ x → x = y := by apply F.rel_antisymm
 
 end Frame
 
-abbrev pointFrame : Frame where
+structure FiniteFrame extends Frame where
+  [world_finite : Finite World]
+attribute [simp] FiniteFrame.world_finite
+
+def Frame.toFinite (F : Frame) [Finite F.World] : FiniteFrame := ⟨F⟩
+
+section
+
+abbrev whitepoint : FiniteFrame where
   World := Unit
   Rel := fun _ _ => True
   rel_refl := by simp [Reflexive]
   rel_trans := by simp [Transitive]
   rel_antisymm := by simp [AntiSymmetric]
 
+end
+
+
 abbrev FrameClass := Set (Frame)
+
+abbrev FiniteFrameClass := Set (FiniteFrame)
+
+def FiniteFrameClass.toFrameClass (C : FiniteFrameClass) : FrameClass := C.image (·.toFrame)
+
+lemma exists_finiteFrameClass_of_mem_toFrameClass {C : FiniteFrameClass} (hF : F ∈ C.toFrameClass) : ∃ F' ∈ C, F'.toFrame = F := by
+  simpa [FiniteFrameClass.toFrameClass] using hF;
+
 
 structure Valuation (F : Frame) where
   Val : F.World → ℕ → Prop
@@ -298,6 +317,9 @@ protected lemma efq : F ⊧ Axioms.EFQ φ := fun _ => ValidOnModel.efq
 
 end ValidOnFrame
 
+instance : Semantics (Formula ℕ) Kripke.FiniteFrame := ⟨fun F => Formula.Kripke.ValidOnFrame F.toFrame⟩
+@[simp] lemma ValidOnFiniteFrame.iff_ValidOnFrame {F : Kripke.FiniteFrame} : F ⊧ φ ↔ F.toFrame ⊧ φ := iff_of_eq rfl
+
 end Formula.Kripke
 
 
@@ -328,6 +350,31 @@ alias ⟨exists_model_world_of_not_validOnFrameClass, not_validOnFrameClass_of_e
 
 end
 
+
+section
+
+variable {C : FiniteFrameClass} {φ ψ χ : Formula ℕ}
+
+lemma iff_validOnFiniteFrameClass_validOnModel : (C ⊧ φ) ↔ (∀ M : Model, ∀ x : M.World, (M_finite : Finite M.toFrame) → M.toFrame.toFinite ∈ C → x ⊧ φ) := by
+  constructor;
+  . intro hF M x M_fin M_C;
+    apply @hF M.toFrame.toFinite M_C;
+  . intro h F hF V x;
+    apply @h ⟨F.toFrame, V⟩ x ?_ ?_;
+    . exact F.world_finite;
+    . tauto;
+
+alias ⟨validOnModel_of_validOnFiniteFrameClass, validOnFiniteFrameClass_of_validOnModel⟩ := iff_validOnFiniteFrameClass_validOnModel
+
+lemma iff_not_validOnFiniteFrameClass_exists_finiteFrame : (¬C ⊧ φ) ↔ (∃ F ∈ C, ¬F ⊧ φ) := by
+  apply not_iff_not.mp;
+  push_neg;
+  tauto;
+alias ⟨exists_finiteFrame_of_not_validOnFiniteFrameClass, not_validOnFiniteFrameClass_of_exists_finiteFrame⟩ := iff_not_validOnFiniteFrameClass_exists_finiteFrame
+
+end
+
+
 namespace FrameClass
 
 variable {C : FrameClass} {φ ψ χ : Formula ℕ}
@@ -335,14 +382,7 @@ variable {C : FrameClass} {φ ψ χ : Formula ℕ}
 class DefinedBy (C : Kripke.FrameClass) (Γ : Set (Formula ℕ)) where
   defines : ∀ F, F ∈ C ↔ (∀ φ ∈ Γ, F ⊧ φ)
 
-class FiniteDefinedBy (C Γ) extends FrameClass.DefinedBy C Γ where
-  finite : Set.Finite Γ
-
 abbrev DefinedByFormula (C : Kripke.FrameClass) (φ : Formula ℕ) := FrameClass.DefinedBy C {φ}
-
-lemma definedByFormula_of_iff_mem_validate (h : ∀ F, F ∈ C ↔ F ⊧ φ) : DefinedByFormula C φ := by
-  constructor;
-  simpa;
 
 instance definedBy_inter
   (C₁ Γ₁) [h₁ : DefinedBy C₁ Γ₁]
@@ -376,17 +416,70 @@ instance definedByFormula_inter
 end FrameClass
 
 
+namespace FiniteFrameClass
+
+class DefinedBy (C : Kripke.FiniteFrameClass) (Γ : Set (Formula ℕ)) where
+  defines : ∀ F, F ∈ C ↔ (∀ φ ∈ Γ, F ⊧ φ)
+
+abbrev DefinedByFormula (C : Kripke.FiniteFrameClass) (φ : Formula ℕ) := FiniteFrameClass.DefinedBy C {φ}
+
+instance definedBy_inter
+  (C₁ Γ₁) [h₁ : DefinedBy C₁ Γ₁]
+  (C₂ Γ₂) [h₂ : DefinedBy C₂ Γ₂]
+  : DefinedBy (C₁ ∩ C₂) (Γ₁ ∪ Γ₂) := ⟨by
+  rintro F;
+  constructor
+  . rintro ⟨hF₁, hF₂⟩;
+    rintro φ (hφ₁ | hφ₂);
+    . exact h₁.defines F |>.mp hF₁ _ hφ₁;
+    . exact h₂.defines F |>.mp hF₂ _ hφ₂;
+  . intro h;
+    constructor;
+    . apply h₁.defines F |>.mpr;
+      intro φ hφ;
+      apply h;
+      left;
+      assumption;
+    . apply h₂.defines F |>.mpr;
+      intro φ hφ;
+      apply h;
+      right;
+      assumption;
+⟩
+
+instance definedByFormula_inter
+  (C₁ φ₁) [DefinedByFormula C₁ φ₁]
+  (C₂ φ₂) [DefinedByFormula C₂ φ₂]
+  : DefinedBy (C₁ ∩ C₂) {φ₁, φ₂} := definedBy_inter C₁ {φ₁} C₂ {φ₂}
+
+end FiniteFrameClass
+
+
 protected abbrev FrameClass.all : FrameClass := Set.univ
 
-instance : FrameClass.all.DefinedByFormula (Axioms.EFQ (.atom 0)) :=
-  FrameClass.definedByFormula_of_iff_mem_validate $ by
-    simp only [Set.mem_univ, true_iff];
-    intro F;
-    exact Formula.Kripke.ValidOnFrame.efq;
+instance : FrameClass.all.DefinedByFormula (Axioms.EFQ (.atom 0)) := ⟨by
+  simp only [Set.mem_univ, Set.mem_singleton_iff, Kripke.ValidOnFrame.models_iff, forall_eq, true_iff];
+  intro F;
+  exact Formula.Kripke.ValidOnFrame.efq;
+⟩
 
 @[simp]
 instance : FrameClass.all.Nonempty := by
-  use pointFrame;
+  use whitepoint.toFrame;
+  trivial;
+
+
+abbrev FiniteFrameClass.all : FiniteFrameClass := Set.univ
+
+instance : FiniteFrameClass.all.DefinedByFormula (Axioms.EFQ (.atom 0)) := ⟨by
+  simp only [Set.mem_univ, Set.mem_singleton_iff, Kripke.ValidOnFrame.models_iff, forall_eq, true_iff];
+  intro F;
+  exact Formula.Kripke.ValidOnFrame.efq;
+⟩
+
+@[simp]
+instance : FiniteFrameClass.all.Nonempty := by
+  use whitepoint;
   trivial;
 
 
