Foundation/Propositional/Logic/Basic.lean
@@ -54,6 +54,11 @@ section
 open Kripke
 
 abbrev Kripke.FrameClass.logic (C : FrameClass) : Logic := { φ | C ⊧ φ }
+abbrev Kripke.FiniteFrameClass.logic (C : FiniteFrameClass) : Logic := { φ | C ⊧ φ }
+
+@[simp]
+lemma Logic.eq_kripkeFiniteFrameClass_toFrameClas_logic {C : Kripke.FiniteFrameClass} : (C.toFrameClass.logic) = C.logic := by
+  simp [Kripke.FiniteFrameClass.logic, Kripke.FrameClass.logic, FiniteFrameClass.toFrameClass, Semantics.Realize]
 
 lemma Logic.eq_Hilbert_Logic_KripkeFrameClass_Logic {H : Hilbert ℕ} {C : FrameClass}
   [sound : Sound H C] [complete : Complete H C]
@@ -63,9 +68,17 @@ lemma Logic.eq_Hilbert_Logic_KripkeFrameClass_Logic {H : Hilbert ℕ} {C : Frame
   . exact sound.sound;
   . exact complete.complete;
 
+lemma Logic.eq_Hilbert_Logic_KripkeFiniteFrameClass_Logic {H : Hilbert ℕ} {C : FiniteFrameClass}
+  [sound : Sound H C] [complete : Complete H C]
+  : H.logic = C.logic := by
+  ext φ;
+  constructor;
+  . exact sound.sound;
+  . exact complete.complete;
+
 lemma Logic.Int.Kripke.eq_all : Logic.Int = FrameClass.all.logic := eq_Hilbert_Logic_KripkeFrameClass_Logic
 
-lemma Logic.Int.Kripke.eq_all_finite : Logic.Int = Kripke.FrameClass.all_finite.logic := eq_Hilbert_Logic_KripkeFrameClass_Logic
+lemma Logic.Int.Kripke.eq_all_finite : Logic.Int = Kripke.FiniteFrameClass.all.logic := eq_Hilbert_Logic_KripkeFiniteFrameClass_Logic
 
 end
 
